Improved the proof tactic for predicate to support (de)atomisation of quantifiers. Also completed support for this proof tactic in other theories. Finally, removed the explicit definition for the algebraic version of sequential composition and made some minor cosmetic changes to utp_subst.

theories/tactics/utp_pred_tac.thy
@@ -134,6 +134,10 @@ apply (simp add: ForallP_def)
 apply (simp add: EvalP_NotP EvalP_ExistsP closure)
 done
 
+theorems EvalP_QuantP =
+  EvalP_ExistsP
+  EvalP_ForallP
+
 theorem EvalP_ClosureP [eval] :
 "\<lbrakk>p \<in> WF_PREDICATE;
  b \<in> WF_BINDING\<rbrakk> \<Longrightarrow>
@@ -154,51 +158,125 @@ done
 declare Tautology_def [eval]
 declare Contradiction_def [eval]
 declare Refinement_def [eval]
-end
 
-context PRED
-begin
-theorem WF_BINDING_type [intro] :
-"\<lbrakk>b \<in> WF_BINDING\<rbrakk> \<Longrightarrow> (b v) : (type v)"
-apply (simp add: WF_BINDING_def)
-done
+subsection {* Support Theorems *}
 
-theorem WF_BINDING_update [intro] :
-"\<lbrakk>b \<in> WF_BINDING; x : (type v)\<rbrakk> \<Longrightarrow>
- b(v := x) \<in> WF_BINDING"
-apply (simp add: WF_BINDING_def)
-done
-
-theorem Exists_WF_BINDING_override_single :
-"\<lbrakk>b \<in> WF_BINDING\<rbrakk> \<Longrightarrow>
- (\<exists> b' \<in> WF_BINDING . f (b \<oplus> b' on {v})) =
- (\<exists> x \<in> carrier (type v) . f (b(v := x)))"
-apply (simp add: override_on_singleton)
+theorem EvalP_ExistsP_singleton :
+"\<lbrakk>p \<in> WF_PREDICATE;
+ b \<in> WF_BINDING\<rbrakk> \<Longrightarrow>
+ \<lbrakk>\<exists>p {x} . p\<rbrakk>b = (\<exists> v \<in> carrier (type x) . \<lbrakk>p\<rbrakk>(b(x := v)))"
+apply (simp add: ExistsP_def)
+apply (simp add: EvalP_def)
 apply (safe)
-apply (rule_tac x = "b' v" in bexI)
-apply (assumption)
-apply (unfold carrier_def)
-apply (auto) [1]
-apply (rule_tac x = "b(v := x)" in bexI)
-apply (simp)
+-- {* Subgoal 1 *}
+apply (rule_tac x = "b1 x" in bexI)
+apply (simp add: override_on_singleton)
+apply (simp add: WF_BINDING_app_carrier)
+-- {* Subgoal 2 *}
+apply (rule_tac x = "b(x := v)" in exI)
+apply (rule_tac x = "b" in exI)
+apply (simp add: override_on_singleton)
+done
+
+theorem EvalP_ForallP_singleton :
+"\<lbrakk>p \<in> WF_PREDICATE;
+ b \<in> WF_BINDING\<rbrakk> \<Longrightarrow>
+ \<lbrakk>\<forall>p {x} . p\<rbrakk>b = (\<forall> v \<in> carrier (type x) . \<lbrakk>p\<rbrakk>(b(x := v)))"
+apply (simp add: ForallP_def)
+apply (simp add: EvalP_NotP EvalP_ExistsP_singleton closure)
+done
+
+theorems EvalP_QuantP_singleton =
+  EvalP_ExistsP_singleton
+  EvalP_ForallP_singleton
+
+subsection {* Normalisation *}
+
+theorem NotP_NotP :
+"p \<in> WF_PREDICATE \<Longrightarrow>
+ \<not>p \<not>p p = p"
+apply (auto simp: NotP_def)
+done
+
+theorem ExistsP_empty :
+"p \<in> WF_PREDICATE \<Longrightarrow>
+ (\<exists>p {} . p) = p"
+apply (simp add: ExistsP_def)
 apply (auto)
 done
 
-theorem Forall_WF_BINDING_override_single :
-"\<lbrakk>b \<in> WF_BINDING\<rbrakk> \<Longrightarrow>
- (\<forall> b' \<in> WF_BINDING . f (b \<oplus> b' on {v})) =
- (\<forall> x \<in> carrier (type v) . f (b(v := x)))"
-apply (simp add: override_on_singleton)
-apply (safe)
-apply (drule_tac x = "b(v := x)" in bspec)
-apply (unfold carrier_def)
-apply (auto) [1]
-apply (simp)
-apply (drule_tac x = "b' v" in bspec)
-apply (auto) [1]
-apply (assumption)
+theorem ForallP_empty :
+"p \<in> WF_PREDICATE \<Longrightarrow>
+ (\<forall>p {} . p) = p"
+apply (simp add: ForallP_def)
+apply (simp add: ExistsP_empty closure)
+apply (simp add: NotP_NotP)
 done
-end
+
+theorem ExistsP_insert :
+"p \<in> WF_PREDICATE \<Longrightarrow>
+ (\<exists>p (insert v vs) . p) = (\<exists>p {v} . (\<exists>p vs . p))"
+apply (simp add: ExistsP_def [of "(\<exists>p vs . p)"] closure)
+apply (simp add: ExistsP_def)
+apply (safe)
+-- {* Subgoal 1 *}
+apply (rule_tac x = "b1 \<oplus> b2 on vs" in exI)
+apply (rule_tac x = "b2" in exI)
+apply (simp)
+apply (rule_tac x = "b1" in exI)
+apply (rule_tac x = "b2" in exI)
+apply (simp)
+-- {* Subgoal 2 *}
+apply (rule_tac x = "b1a" in exI)
+apply (rule_tac x = "b2a \<oplus> b2 on {v}" in exI)
+apply (simp)
+apply (simp add: override_on_assoc closure)
+done
+
+theorem ForallP_insert :
+"p \<in> WF_PREDICATE \<Longrightarrow>
+ (\<forall>p (insert v vs) . p) = (\<forall>p {v} . (\<forall>p vs . p))"
+apply (simp add: ForallP_def closure)
+apply (simp add: NotP_NotP closure)
+apply (subst ExistsP_insert)
+apply (simp_all add: closure)
+done
+
+theorem ExistsP_atomise :
+"p \<in> WF_PREDICATE \<Longrightarrow>
+ (\<exists>p {x} . (\<exists>p (insert y vs) . p)) =
+ (\<exists>p (insert x (insert y vs)) . p)"
+apply (auto intro!: sym [OF ExistsP_insert])
+done
+
+theorem ForallP_atomise :
+"p \<in> WF_PREDICATE \<Longrightarrow>
+ (\<forall>p {x} . (\<forall>p (insert y vs) . p)) =
+ (\<forall>p (insert x (insert y vs)) . p)"
+apply (auto intro!: sym [OF ForallP_insert])
+done
+
+theorems QuantP_atomise =
+  ExistsP_atomise
+  ForallP_atomise
+
+theorem ExistsP_deatomise :
+"p \<in> WF_PREDICATE \<Longrightarrow>
+ (\<exists>p (insert x (insert y vs)) . p) =
+ (\<exists>p {x} . (\<exists>p (insert y vs) . p))"
+apply (auto intro!: ExistsP_insert)
+done
+
+theorem ForallP_deatomise :
+"p \<in> WF_PREDICATE \<Longrightarrow>
+ (\<forall>p (insert x (insert y vs)) . p) =
+ (\<forall>p {x} . (\<forall>p (insert y vs) . p))"
+apply (auto intro!: ForallP_insert)
+done
+
+theorems QuantP_deatomise =
+  ExistsP_deatomise
+  ForallP_deatomise
 
 subsection {* Proof Tactics *}
 
@@ -215,27 +293,81 @@ ML {*
 *}
 
 ML {*
-  fun utp_pred_auto_simpset ctxt =
+  fun utp_atomise_simpset ctxt =
     (simpset_of ctxt)
+      addsimps @{thms QuantP_atomise}
+      addsimps (closure.get ctxt);
+*}
+
+ML {*
+  fun utp_deatomise_simpset ctxt =
+    (simpset_of ctxt)
+      addsimps @{thms QuantP_deatomise}
+      addsimps (closure.get ctxt);
+*}
+
+ML {*
+  fun utp_singleton_simpset ctxt =
+    (simpset_of ctxt)
+      addsimps (eval.get ctxt)
+      delsimps @{thms EvalP_QuantP}
+      addsimps @{thms EvalP_QuantP_singleton}
+      addsimps (closure.get ctxt);
+*}
+
+ML {*
+  fun utp_auto_simpset ctxt =
+    (simpset_of ctxt);
 *}
 
 ML {*
   fun utp_pred_tac thms ctxt i =
-    CHANGED (asm_full_simp_tac (utp_pred_simpset ctxt) i)
+    CHANGED (
+      TRY (asm_full_simp_tac (utp_pred_simpset ctxt) i))
 *}
 
 ML {*
-  fun utp_pred_auto_tac thms ctxt i =
-    TRY (asm_full_simp_tac (utp_pred_simpset ctxt) i) THEN
-    TRY (asm_full_simp_tac (utp_pred_auto_simpset ctxt) i) THEN
-    (auto_tac ctxt)
+  fun utp_pred_atomise_tac thms ctxt i =
+    CHANGED (
+      TRY (asm_full_simp_tac (utp_atomise_simpset ctxt) i) THEN
+      TRY (asm_full_simp_tac (utp_pred_simpset ctxt) i))
 *}
+
+ML {*
+  fun utp_pred_deatomise_tac thms ctxt i =
+    CHANGED (
+      TRY (asm_full_simp_tac (utp_deatomise_simpset ctxt) i) THEN
+      TRY (asm_full_simp_tac (utp_singleton_simpset ctxt) i))
+*}
+
+text {* Should we atomise or deatomise below? *}
+
+ML {*
+  fun utp_pred_auto_tac thms ctxt i =
+    CHANGED  (
+      TRY (asm_full_simp_tac (utp_pred_simpset ctxt) i) THEN
+      TRY (asm_full_simp_tac (utp_auto_simpset ctxt) i) THEN
+      (auto_tac ctxt))
+*}
+end
 
 method_setup utp_pred_tac = {*
   Attrib.thms >>
   (fn thms => fn ctxt =>
     SIMPLE_METHOD' (utp_pred_tac thms ctxt))
 *} "proof tactic for predicates"
+
+method_setup utp_pred_atomise_tac = {*
+  Attrib.thms >>
+  (fn thms => fn ctxt =>
+    SIMPLE_METHOD' (utp_pred_atomise_tac thms ctxt))
+*} "proof tactic for predicates with atomisation"
+
+method_setup utp_pred_deatomise_tac = {*
+  Attrib.thms >>
+  (fn thms => fn ctxt =>
+    SIMPLE_METHOD' (utp_pred_deatomise_tac thms ctxt))
+*} "proof tactic for predicates with deatomisation"
 
 method_setup utp_pred_auto_tac = {*
   Attrib.thms >>
@@ -247,6 +379,15 @@ subsection {* Proof Experiments *}
 
 context PRED
 begin
+
+theorem ExistsP_norm_test :
+"p \<in> WF_PREDICATE \<Longrightarrow>
+ (\<exists>p {x} . \<exists>p {y} . p) = (\<exists>p {y} . \<exists>p {x} . p)"
+apply (utp_pred_atomise_tac)
+apply (subgoal_tac "{x, y} = {y, x}")
+apply (simp)
+apply (auto)
+done
 
 theorem AndP_assoc :
 "\<lbrakk>p1 \<in> WF_PREDICATE;
@@ -276,20 +417,20 @@ theorem AndP_comm_taut :
 apply (utp_pred_auto_tac)
 done
 
-theorem AndP_eq_FalseP :
+theorem AndP_equals_FalseP :
 "\<lbrakk>p \<in> WF_PREDICATE\<rbrakk> \<Longrightarrow>
  p \<and>p \<not>p p = false"
 apply (utp_pred_auto_tac)
 done
 
-theorem OrP_eq_TrueP :
+theorem OrP_equals_TrueP :
 "\<lbrakk>p \<in> WF_PREDICATE;
  a \<in> WF_ALPHABET\<rbrakk> \<Longrightarrow>
  p \<or>p \<not>p p = true"
 apply (utp_pred_auto_tac)
 done
 
-theorem ForallP_NotP_taut :
+theorem ForallP_NotP_ExistsP_taut :
 "\<lbrakk>p \<in> WF_PREDICATE\<rbrakk> \<Longrightarrow>
  taut (\<forall>p vs . \<not>p p) \<Leftrightarrow>p \<not>p (\<exists>p vs . p)"
 apply (utp_pred_auto_tac)
